complete proofs of derived rules

iris_derived_rules.v
@@ -14,9 +14,7 @@ Module Type IRIS_DERIVED_RULES (RL : VIRA_T) (C : CORE_LANG) (R: IRIS_RES RL C) 
   Local Open Scope bi_scope.
   Local Open Scope iris_scope.
 
-  (* Ideally, these rules should never talk about worlds or such.
-     At the very least, they should not open the definition of the complex assertions:
-     invariants, primitive view shifts, weakest pre. *)
+  (* These rules and their proofs should never talk about worlds or step-indices. *)
 
   Section DerivedVSRules.
 
@@ -161,7 +159,7 @@ Module Type IRIS_DERIVED_RULES (RL : VIRA_T) (C : CORE_LANG) (R: IRIS_RES RL C) 
       vs m1 m2 P Q ⊑ vs (m1 ∪ mf) (m2 ∪ mf) (P * R) (Q * R).
     Proof.
       move=>H. rewrite {1}/vs. apply vsIntro.
-      etransitivity; last eapply pvsFrameRes.
+      etransitivity; last by eapply pvsFrameRes.
       etransitivity; last first.
       { eapply sc_pord; last reflexivity. eapply pvsFrameMask. assumption. }
       rewrite -box_conj_star assoc. apply sc_pord; last reflexivity.
@@ -172,35 +170,43 @@ Module Type IRIS_DERIVED_RULES (RL : VIRA_T) (C : CORE_LANG) (R: IRIS_RES RL C) 
 
   Section DerivedHTRules.
 
-    Existing Instance LP_isval.
-
     Implicit Types (P : Props) (i : nat) (m : DecEnsemble nat) (e : expr) (r : res) (φ Q : vPred) (w : Wld) (n k : nat).
 
     Lemma htIntro R safe m e P Q:
       □R ⊑ ht safe m P e Q <-> □R ∧ P ⊑ wp safe m e Q.
     Proof.
       split=>H.
-      - unfold vs in H.
+      - unfold ht in H.
         apply and_impl. etransitivity; last by eapply box_elim. assumption.
-      - unfold vs; apply box_intro. rewrite <-and_impl. assumption.
+      - unfold ht; apply box_intro. rewrite <-and_impl. assumption.
     Qed.
 
     Lemma htValid safe m e P Q:
-      valid (ht safe m P e Q) <-> P ⊑ ht safe m e Q.
+      valid (ht safe m P e Q) <-> P ⊑ wp safe m e Q.
     Proof.
       rewrite ->top_valid, box_top. split=>H.
-      - etransitivity; last by erewrite <-vsIntro. apply and_R; split; last reflexivity.
+      - etransitivity; last by erewrite <-htIntro. apply and_R; split; last reflexivity.
         rewrite <-box_top. apply top_true.
-      - etransitivity; first apply vsIntro; last reflexivity.
+      - etransitivity; first apply htIntro; last reflexivity.
         rewrite <-H. apply and_projR.
     Qed.
 
+    Lemma wpImpl safe m e φ φ':
+      (□all (lift_bin BI.impl φ φ')) ∧ wp safe m e φ ⊑ wp safe m e φ'.
+    Proof.
+      rewrite -box_conj_star comm. rewrite ->wpFrameRes. eapply wpMon.
+      move=>v. rewrite /lift_bin [box]lock /= /const /= -lock.
+      rewrite comm box_conj_star.
+      eapply modus_ponens; first by apply and_projR.
+      etransitivity; first by apply and_projL.
+      etransitivity; first by apply box_elim.
+      apply (all_L v). reflexivity.
+    Qed.
 
     Lemma htRet e (HV : is_value e) safe m :
       valid (ht safe m ⊤ e (eqV (exist _ e HV))).
     Proof.
-      move=>w0 n0 _ w1 Hw01 n1 r1 Hn01 _ _.
-      eapply wpRet.
+      apply htValid. apply top_valid. apply wpRet.
     Qed.
     
     (** Quantification in the logic works over nonexpansive maps, so
@@ -210,23 +216,34 @@ Module Type IRIS_DERIVED_RULES (RL : VIRA_T) (C : CORE_LANG) (R: IRIS_RES RL C) 
       n[(fun v : value => ht safe m (Q v) (fill K v) Q' )].
     Next Obligation.
       intros v1 v2 EQv; unfold ht; eapply (met_morph_nonexp box).
-      eapply (impl_dist (ComplBI := Props_BI)).
+      eapply impl_dist.
       - apply Q; assumption.
-      - destruct n as [| n]; [apply dist_bound | simpl in EQv].
+      - destruct n as [| n]; [apply dist_bound | hnf in EQv].
+        rewrite EQv; reflexivity.
+    Qed.
+
+    Program Definition plugCtxWp safe m Q Q' K :=
+      n[(fun v : value => Q v → wp safe m (fill K v) Q' )].
+    Next Obligation.
+      intros v1 v2 EQv. eapply impl_dist.
+      - apply Q; assumption.
+      - destruct n as [| n]; [apply dist_bound | hnf in EQv].
         rewrite EQv; reflexivity.
     Qed.
 
     Lemma htBind P Q R K e safe m :
       ht safe m P e Q ∧ all (plugCtxHt safe m Q R K) ⊑ ht safe m P (fill K e) R.
     Proof.
-      move=>w0 n0 r0 [He HK] w1 Hw01 n1 r1 Hn01 _ HP.
-      eapply wpBind. eapply wpImpl. split; last first.
-      - unfold ht in He. specialize (He _ Hw01 _ _ Hn01 unit_min HP). eexact He. (* Why does eapply He not work? *)
-      - intros v w2 Hw12 n2 r2 Hn12 _ HQ. simpl. unfold plugCtxHt in HK.
-        move:HK. move/(_ v _ _ _ _ _ _ HQ)=>HK. apply HK. (* TODO: Nicer way to get these as goals (not requiring the current goal to match)? *)
-        + etransitivity; eassumption.
-        + omega.
-        + apply: unit_min.
+      rewrite /plugCtxHt {1 2}/ht. etransitivity; last eapply htIntro.
+      { erewrite box_conj. apply and_pord; first reflexivity.
+        apply pordR. symmetry. erewrite (box_all (plugCtxWp safe m Q R K)). unfold box_all_lhs. apply all_equiv=>v.
+        reflexivity. }
+      etransitivity; last by eapply wpBind.
+      etransitivity; last eapply wpImpl with (φ:=Q). apply and_R; split.
+      - rewrite ->and_projL. apply box_intro. rewrite ->box_elim, ->and_projR.
+        apply all_pord=>v. reflexivity.
+      - eapply modus_ponens; first by apply and_projR.
+        rewrite ->and_projL, ->box_elim. apply and_projL.
     Qed.
 
     (** Much like in the case of the plugging, we need to show that
@@ -239,92 +256,111 @@ Module Type IRIS_DERIVED_RULES (RL : VIRA_T) (C : CORE_LANG) (R: IRIS_RES RL C) 
       rewrite ->EQv; reflexivity.
     Qed.
 
+    Program Definition pvsLift m1 m2 (φ φ' : vPred) :=
+      n[(fun v => φ v → pvs m1 m2 (φ' v))].
+    Next Obligation.
+      intros v1 v2 EQv. apply impl_dist; first now rewrite EQv.
+      apply (met_morph_nonexp (pvs m1 m2)). now rewrite EQv.
+    Qed.
+
     Lemma pvsWpCompose {safe m m' P e φ}:
       pvs m m' P ∧ ht safe m' P e φ ⊑ pvs m m' (wp safe m' e φ).
     Proof.
-      move=>w0 n0 r0 [Hpvs Hht]. unfold vsLift, vs, ht in *.
-      eapply pvsImpl. split; eassumption.
+      rewrite /ht comm. etransitivity; first by apply pvsImpl.
+      apply pvsMon. reflexivity.
+    Qed.
+
+    Lemma vsLiftBox m' m φ φ':
+      □all (pvsLift m' m φ φ') == all (vsLift m' m φ φ').
+    Proof.
+      etransitivity; first by eapply (box_all (pvsLift m' m φ φ')).
+      unfold box_all_lhs. apply all_equiv=>v. reflexivity.
     Qed.
 
     Lemma wpPvsCompose {safe m m' e φ φ'}:
       wp safe m' e φ ∧ all (vsLift m' m φ φ') ⊑ wp safe m' e (pvs m' m <M< φ').
     Proof.
-      move=>w0 n0 r0 [Hwp Hvs]. unfold vsLift, vs, ht in *.
-      eapply wpImpl. split; last eassumption.
-      move=>v w1 Hw01 n1 r1 Hn01 _ Hφ. change (pvs m' m (φ' v) w1 n1 r1).
-      specialize (Hvs v). apply: Hvs Hφ; [assumption|by apply:unit_min].
+      rewrite -vsLiftBox /vs.
+      rewrite comm. etransitivity; last by apply wpImpl.
+      eapply and_pord; last reflexivity. apply pordR.
+      apply morph_resp. apply all_equiv=>v. reflexivity.
     Qed.
 
     Lemma htCons P P' Q Q' safe m e :
       vs m m P P' ∧ ht safe m P' e Q' ∧ all (vsLift m m Q' Q) ⊑ ht safe m P e Q.
     Proof.
-      move=>w0 n0 r0 [HvsP [Hht HvsQ]] w1 Hw01 n1 r1 Hn01 _ HP.
-      eapply wpPostVS, wpPvsCompose. split; last first.
-      { eapply propsMWN; last apply: HvsQ; assumption. }
-      eapply wpPreVS, pvsWpCompose. split; last first.
-      { eapply propsMWN; last apply: Hht; assumption. }
-      unfold vs in HvsP=>{Hht HvsQ}. eapply HvsP; (assumption || by apply: unit_min).
+      rewrite /vs {1}/ht -vsLiftBox -!box_conj. apply htIntro.
+      etransitivity; last by eapply wpPostVS.
+      etransitivity; last by eapply wpPvsCompose. apply and_R; split; last first.
+      - rewrite ->and_projL, !box_conj, vsLiftBox, !and_projR. reflexivity.
+      - etransitivity; last by eapply wpPreVS.
+        etransitivity; last by eapply pvsWpCompose. apply and_R; split.
+        + eapply modus_ponens; last first.
+          * rewrite ->box_elim, !and_projL. reflexivity.
+          * apply and_projR.
+        + rewrite /ht. rewrite ->and_projL. apply box_intro.
+          rewrite ->box_elim, and_projR, and_projL. reflexivity.
     Qed.
 
     Lemma htACons safe m m' e P P' Q Q'
           (HAt   : atomic e)
-          (HSub  : m' ⊆ m) :
+          (HSub  : m' ⊑ m) :
       vs m m' P P' ∧ ht safe m' P' e Q' ∧ all (vsLift m' m Q' Q) ⊑ ht safe m P e Q.
     Proof.
-      move=>w0 n0 r0 [HvsP [Hht HvsQ]] w1 Hw01 n1 r1 Hn01 _ HP.
-      unfold vsLift, vs, ht in *.
-      eapply wpACons;[eassumption|eassumption|].
-      eapply pvsWpCompose. split.
-      { apply: HvsP; (assumption || by apply: unit_min). }
-      move=>w2 Hw12 n2 r2 Hn12 Hr12 HP'.
-      eapply wpPvsCompose. split; last first.
-      { eapply propsMWN; last apply: HvsQ; (etransitivity;eassumption). }
-      (* TODO: This next step is slow. It's still the most sensible script though. *)
-      eapply Hht, HP'; ((etransitivity;eassumption) || by apply: unit_min).
+      rewrite /vs {1}/ht -vsLiftBox -!box_conj. apply htIntro.
+      etransitivity; last (eapply wpACons; eassumption).
+      etransitivity; last eapply pvsWpCompose. apply and_R; split.
+      - eapply modus_ponens.
+        + apply and_projR.
+        + rewrite ->and_projL, box_elim, !and_projL. reflexivity.
+      - rewrite ->and_projL. apply htIntro.
+        etransitivity; last eapply wpPvsCompose. apply and_R; split; last first.
+        + erewrite <-vsLiftBox, and_projL. apply box_intro.
+          rewrite ->box_elim, !and_projR. reflexivity.
+        + eapply modus_ponens; first by apply and_projR.
+          rewrite ->and_projL, box_elim, and_projR. apply and_projL.
     Qed.
 
     Lemma htFrame safe m m' P R e Q (HD : m # m') :
       ht safe m P e Q ⊑ ht safe (m ∪ m') (P * R) e (lift_bin sc Q (umconst R)).
     Proof.
-      move=>w0 n0 r0 Hht w1 Hw01 n1 r1 Hn01 _ [r1_1 [r1_2 [HEQr [HP HR]]]].
-      eapply wpFrameMask; first by assumption.
-      eapply wpFrameRes. exists r1_1 r1_2. split; first assumption. split.
-      - unfold ht in Hht. specialize (Hht _ Hw01 _ _ Hn01 unit_min HP). assumption.
-      - assumption.
+      rewrite {1}/ht. apply htIntro.
+      etransitivity; last by eapply wpFrameRes.
+      etransitivity; last first.
+      { eapply sc_pord; last reflexivity. eapply wpFrameMask. assumption. }
+      rewrite -box_conj_star assoc. apply sc_pord; last reflexivity.
+      rewrite box_conj_star. apply and_impl, box_elim.
     Qed.
-
+      
     Lemma htAFrame safe m m' P R e Q
           (HD  : m # m')
           (HAt : atomic e) :
       ht safe m P e Q ⊑ ht safe (m ∪ m') (P * ▹R) e (lift_bin sc Q (umconst R)).
     Proof.
-      move=>w0 n0 r0 Hht w1 Hw01 n1 r1 Hn01 _ [r1_1 [r1_2 [HEQr [HP HLR]]]].
-      eapply wpFrameMask; first by assumption.
-      eapply wpAFrameRes; first assumption. exists r1_1 r1_2. split; first assumption. split.
-      - unfold ht in Hht. specialize (Hht _ Hw01 _ _ Hn01 unit_min HP). assumption.
-      - assumption.
+      rewrite {1}/ht. apply htIntro.
+      etransitivity; last (eapply wpAFrameRes; assumption).
+      etransitivity; last first.
+      { eapply sc_pord; last reflexivity. eapply wpFrameMask. assumption. }
+      rewrite -box_conj_star assoc. apply sc_pord; last reflexivity.
+      rewrite box_conj_star. apply and_impl, box_elim.
     Qed.
 
     Lemma htFork safe m P R e :
       ht safe m P e (umconst ⊤) ⊑ ht safe m (▹P * ▹R) (fork e) (lift_bin sc (eqV (exist _ fork_ret fork_ret_is_value)) (umconst R)).
     Proof.
-      move=>w0 n0 r0 Hht w1 Hw01 n1 r1 Hn01 _ [r1_1 [r1_2 [HEQr [HLP HLR]]]].
-      eapply wpFork. exists r1_1 r1_2. split; first assumption. split.
-      - eapply laterM. split; last by eapply HLP. move=> w2 Hw12 n2 r2 Hn12 Hr12 HP.
-        move:Hht. move/(_ _ _ _ _ _ _ HP)=>{HP}HP. apply HP.
-        + etransitivity; eassumption.
-        + omega.
-        + apply: unit_min.
-      - assumption.
+      rewrite {1}/ht. apply htIntro.
+      etransitivity; last by eapply wpFork.
+      rewrite -box_conj_star assoc. apply sc_pord; last reflexivity.
+      rewrite box_conj_star. apply and_impl. rewrite <-later_impl, ->box_elim.
+      apply later_mon.
     Qed.
 
     Lemma htUnsafe {m P e Q} :
       ht true m P e Q ⊑ ht false m P e Q.
     Proof.
-      move=>w0 n0 r0 Hht w1 Hw01 n1 r1 Hn01 _ HP.
-      eapply wpUnsafe. move:Hht. move/(_ _ _ _ _ _ _ HP)=>{HP}HP. apply HP.
-      + assumption.
-      + apply: unit_min.
+      rewrite {1}/ht. apply htIntro.
+      etransitivity; last by eapply wpUnsafe.
+      rewrite ->box_elim. apply and_impl. reflexivity.
     Qed.
 
   End DerivedHTRules.
